+++
title = 'Generating functions'
description = "ASD HELLO"
date = 2024-05-12T13:26:47+02:00
tags = ["Math", "Combinatorics"]
draft = false
math = true
+++


## Formally:
The generating function of an infinite sequence $(a_0, a_1, \ldots\)$ is represented by the power series:
$$
\sum_{n=0}^\infty a_nx^n
$$

## Informally:
Consider a sequence of numbers $(a_0, a_1, \ldots\)$. We want to encode this sequence within a function, expressed as:
$$
a_0x^0 + a_1x^1 + a_2x^2 + \ldots + a_nx^n = \displaystyle\sum_{n=0}^\infty a_nx^n
$$  

### Example of Sequence $(1, 1, 1, 1, \ldots )$:

$$
1x^0 + 1x^1 + 1x^2 + \ldots + 1x^n = \displaystyle\sum_{n=0}^\infty x^n = \frac{1}{1 - x}
$$

You may ask why the equation $\displaystyle\sum_{n=0}^\infty x^n = \frac{1}{1 - x}$ holds. This is explained by the [convergence of geometric series](https://en.wikipedia.org/wiki/Geometric_series#:~:text=The%20convergence%20of%20the%20geometric%20series%20depends%20on%20the%20value,the%20series%20does%20not%20converge.).

The series:
$$
\sum_{n=0}^\infty x^n
$$ 
is a geometric series with the common ratio \(x\). The sum \(S\) of an infinite geometric series is given by the formula:
$$
S = \frac{a}{1 - r}
$$
where \(a\) is the first term of the series and \(r\) is the common ratio. For this specific series:

- \(a = 1\) (the first term)
- \(r = x\) (the common ratio)

Hence:
$$
\displaystyle\sum_{n=0}^\infty x^n = \frac{1}{1 - x}
$$

## Multiplication of GF's and their combinatorial meaning

Let $A(x) = \sum_{n=0}^\infty a_nx^n$ \
Let $B(x) = \sum_{n=0}^\infty b_nx^n$

Then:
$$
    A(x)B(x) = \sum_{n=0}^\infty (\sum_{i = 0}^n a_ib_{n-i})x^n
$$

Notice that $A(x)B(x)$ is the generating function of the sequence with $n$-th element $\sum_{i = 0}^n a_ib_{n-i}$. From combinatorial perspective it's the number of ways you can combine 2 types of objects in a size of n.

Let's have an example for better understaning.

**Problem:** Find number of strings consisting of letters a,b,c of length n not containing `aa` as substring

The hard part is to construct the generatin function, after getting the closed form of it, there are multiple ways to decode it.

So let's let's denote `A` as generating function for `strings not containing aa` and analyize what are the cases we have.

 - empty
 - a
 - b + [strings not containing `aa`] (notice the recursion)
 - c + [strings not containing `aa`]
 - ab + [strings not containtng `aa`]
 - ac + [strings not containing `aa`]

 let's convert those into generating functions.

 - empty = 1
 - a = x
 - b + [strings not containing `aa`] = xA (one element x and rest is recursively generated by A)
 - c + [strings not containing `aa`] = xA (one element x and rest is recursively generated by A)
 - ab + [strings not containtng `aa`] = x^2A (two elements hence x^2 and rest again is recursively generated by A)
 - ac + [strings not containing `aa`] = x^2A similarly to the previous.


 So $A = 1 + x + xA + xA + x^2A + x^2A = 1 + x + 2xA + 2x^2A = \frac{1 + x}{1 - 2x - 2x^2}$

Now we could obtain the exact formula for coefficients of the power series expansion of A. Which would require set of techniques such as `partial fraction decomposition`, explaining which is an another article, but these techniques are completly mechanical, so the hard part is to have the generating function in this form, rest is easy to find.

## References

- [Zdeněk Dvořák. *Notes on combinatorics and graph theory 2*](https://iuuk.mff.cuni.cz/~rakdver/kgii/lesson20-11.pdf).
- [Irena Penev. *Combinatorics and Graph Theory 1 & 2*](https://iuuk.mff.cuni.cz/~ipenev/KGLectureNotes.pdf). Page: 20 